src/Heapsort/ValuePQ.dfy
@@ -1,0 +1,31 @@
+include "../Knapsack/Implementation/PQ.dfy"
+
+module ValuePQ refines PQ {
+
+  class PriorityQueue ... {}
+
+  class Solution ... {
+
+    var value : real
+
+    constructor(value': real)
+      ensures value == value'
+    {
+      value := value';
+    }
+
+    
+    /* Predicados */
+
+    /* 
+    Predicado: define el orden estricto (<) entre dos soluciones.
+    */
+    predicate lt (other : Solution)
+      ensures !other.lt(other)
+    {
+      value < other.value
+    }
+  }
+
+}
+
